Add proofs for get_next_power_of_two.

src/dafny/simpleEth2.0/Merkle.dfy
@@ -39,4 +39,84 @@ module Merkle {
             //  
             b := value == root ;
         } 
+
+    /** Compute 2^n.  */
+    function power2(n : nat): nat 
+    ensures power2(n) >= 1
+    {
+        if n == 0 then 1 else 2 * power2(n - 1)
+    }
+
+    /** Get the next power of two. */
+    function get_next_power_of_two(n : nat) : nat 
+    {
+        if n == 0 then 0
+        else if n <= 2 then n
+        else 2 * get_next_power_of_two( (n + 1) / 2)
+    }
+
+    /** Some desirable properties of get_next_power_of_two.  */
+    lemma lem1(n: nat) 
+        ensures get_next_power_of_two(0) == 1 
+        ensures get_next_power_of_two(1) == 1 
+        ensures get_next_power_of_two(2) == 2 
+        ensures get_next_power_of_two(3) == 2 
+        ensures get_next_power_of_two(8) == 4 
+        ensures get_next_power_of_two(15) == 5 
+        
+    /** Arithmetic 1. */
+    lemma la(n: nat) 
+        requires n >= 2;
+        ensures 2 * (n - 1) >= n {
+        }
+
+    /** Power of two is monotonic. */
+    lemma power2_monotonic(n: nat, n': nat) 
+        requires n > n'
+        ensures n > n' ==> power2(n) > power2(n') {
+
+        }
+
+    /** Lower bound for power2. */
+    lemma lb(n : nat) 
+        ensures power2(n + 1) >= n {
+            if n <= 1 {
+                //  Dafny can infer the proof
+            } else {
+                calc >= {
+                    power2(n + 1) ; 
+                    2 * power2(n)  ;
+                        { lb(n - 1); }
+                    2 * (n - 1);
+                        { la(n) ;}  //  not necessary
+                }
+            }
+        }
+
+    /** Arithmetic equivalence. */
+    lemma k1(x: int, y: int) 
+        ensures x > y / 2 <==> 2 * x > y 
+
+    /** get_next_power_of_two(x) = i, then x < 2^i */
+    lemma lem2(n: nat) 
+        ensures power2(get_next_power_of_two(n)) > n
+        {
+            if n <= 2 { 
+                //  Proof can be infered by Dafny
+            }  
+            else { 
+                calc {
+                    get_next_power_of_two((n + 1)/2) > (n + 1)/2;
+                        ==> { k1( get_next_power_of_two((n + 1)/2), n + 1); }
+                    (2 * get_next_power_of_two((n + 1)/2)) > (n + 1);
+                        ==> { power2_monotonic(2 * get_next_power_of_two((n + 1)/2), n + 1 ); } 
+                    power2(2 * get_next_power_of_two((n + 1)/2)) > power2(n + 1); 
+                        ==> { lb(n); }
+                    power2(2 * get_next_power_of_two((n + 1)/2)) > n  ;
+                        ==>
+                    power2(get_next_power_of_two(n)) > n ;
+                    true;
+                } 
+            }
+        }
 }
